AbsInt.v
@@ -3,63 +3,145 @@ Require Import CSet Le.
 Require Import Plus Util AllInRel Map.
 Require Import Val Var Env EnvTy IL Annotation Lattice DecSolve LengthEq MoreList.
 
-Class AbstractInterpretation Dom FunDom `{SemiLattice Dom} := {
-  transform : list FunDom -> stmt -> ann Dom -> Dom;
-  mkFunDom : params -> ann Dom -> FunDom
+Set Implicit Arguments.
+
+Inductive direction :=
+  Forward | Backward.
+
+Inductive anni (A:Type) : Type :=
+| anni0 : anni A
+| anni1 (a1:A) : anni A
+| anni2 (a1:A) (a2:A) : anni A.
+
+Arguments anni A.
+Arguments anni0 [A].
+
+Fixpoint setAnni {A} (a:ann A) (ai:anni A) : ann A :=
+  match a, ai with
+    | ann1 a an, anni1 a1 => ann1 a (setTopAnn an a1)
+    | ann2 a an1 an2, anni2 a1 a2 => ann2 a (setTopAnn an1 a1) (setTopAnn an2 a2)
+    | an, _ => an
+  end.
+
+Class BackwardAnalysis Dom FunDom `{BoundedSemiLattice Dom} := {
+  btransform : list FunDom -> stmt -> anni Dom -> Dom;
+  bmkFunDom : params -> ann Dom -> FunDom
 }.
 
-Fixpoint backward {Dom} {FunDom} `{SemiLattice Dom} (AI:AbstractInterpretation Dom (FunDom))
+Definition backward Dom FunDom
+           (btransform : list FunDom -> stmt -> anni Dom -> Dom)
+           (bmkFunDom : params -> ann Dom -> FunDom) :=
+  fix backward
          (st:stmt) (AL:list FunDom) (a:ann Dom) {struct st} : ann Dom :=
   match st, a with
     | stmtExp x e s as st, ann1 d ans =>
-      let ans' := backward AI s AL ans in
-      let d' := ann1 d ans' in
-      ann1 (transform AL st d') ans'
+      let ans' := backward s AL ans in
+      let ai := anni1 (getAnn ans') in
+      let d := (btransform AL st ai) in
+      ann1 d ans'
     | stmtIf x s t as st, ann2 d ans ant =>
-      let ans' := backward AI s AL ans in
-      let ant' := backward AI t AL ant in
-      let an' := (ann2 d ans' ant') in
-      ann2 (transform AL st an') ans' ant'
+      let ans' := backward s AL ans in
+      let ant' := backward t AL ant in
+      let ai := anni2 (getAnn ans') (getAnn ant') in
+      let d' := (btransform AL st ai) in
+      ann2 d' ans' ant'
 
     | stmtGoto f Y as st, ann0 d as an =>
-      ann0 (transform AL st an)
+      ann0 (btransform AL st anni0)
 
     | stmtReturn x as st, ann0 d as an =>
-      ann0 (transform AL st an)
+      ann0 (btransform AL st anni0)
 
     | stmtExtern x f Y s as st, ann1 d ans =>
-      let ans' := backward AI s AL ans in
-      let d' := ann1 d ans' in
-      ann1 (transform AL st d') ans'
-
+      let ans' := backward s AL ans in
+      let ai := anni1 (getAnn ans') in
+      let d' := (btransform AL st ai) in
+      ann1 d' ans'
     | stmtLet Z s t as st, ann2 d ans ant =>
-      let ans' := backward AI s (mkFunDom Z ans::AL) ans in
-      let ant' := backward AI t (mkFunDom Z ans'::AL) ant in
-      let d' := ann2 d ans' ant' in
-      ann2 (transform (mkFunDom Z ans'::AL)
-                        st
-                        d') ans' ant'
+      let ans' := backward s (bmkFunDom Z ans::AL) ans in
+      let ant' := backward t (bmkFunDom Z ans'::AL) ant in
+      let ai := anni2 (getAnn ans') (getAnn ant') in
+      let d' := btransform (bmkFunDom Z ans'::AL) st ai in
+      ann2 d' ans' ant'
     | _, an => an
   end.
 
-Set Implicit Arguments.
-Section Analysis.
+
+Definition forward Dom FunDom
+         (ftransform : stmt -> (list FunDom * Dom) -> (list FunDom * anni Dom))
+         (fmkFunDom : params -> ann Dom -> FunDom) :=
+  fix forward
+      (st:stmt) (a:list FunDom * ann Dom) {struct st}
+: list FunDom * ann Dom :=
+  match st, a with
+    | stmtExp x e s as st, (AL, ann1 d ans) =>
+      let (AL', ai) := (ftransform st (AL, d)) in
+      forward s (AL, setAnni ans ai)
+    | stmtIf x s t as st, (AL, ann2 d ans ant) =>
+      let (AL, ai) := (ftransform st (AL, d)) in
+      let (AL', ans') := forward s (AL, setAnni ans ai) in
+      let (AL'', ant') := forward t (AL', setAnni ant ai) in
+      (AL'', ann2 d ans' ant')
+    | stmtGoto f Y as st, (AL, ann0 d as an) =>
+      let (AL', ai) := ftransform st (AL, d) in
+      (AL', an)
+    | stmtReturn x as st, (AL, ann0 d as an) =>
+      let (AL', ai) := ftransform st (AL, d) in
+      (AL', an)
+    | stmtExtern x f Y s as st, (AL, ann1 d ans) =>
+      let (AL, ai) := (ftransform st (AL, d)) in
+      forward s (AL, setAnni ans ai)
+    | stmtLet Z s t as st, (AL, ann2 d ans ant) =>
+      let (AL, ai) := ftransform st (fmkFunDom Z ans::AL, d) in
+      let (AL', ans') := forward s (fmkFunDom Z (setAnni ans ai)::AL, setAnni ans ai) in
+      let (AL'', ant') := forward t (fmkFunDom Z ans'::AL', setAnni ant ai) in
+      (tl AL'', ann2 d ans' ant')
+    | _, an => an
+  end.
+
+Instance PartialOrder_ann Dom `{PartialOrder Dom}
+: PartialOrder (ann Dom) := {
+  poLt := ann_R poLt;
+  poLt_dec := @ann_lt_dec _ _ poLt poLt_dec;
+  poEq := ann_R poEq;
+  poEq_dec := @ann_lt_dec _ _ poEq poEq_dec
+}.
+
+Record Analysis (Dom: Type) := makeAnalysis {
+  dom_po :> PartialOrder Dom;
+  analysis_step : stmt -> Dom -> Dom;
+  initial_value : stmt -> Dom
+}.
+
+Arguments Analysis Dom.
+
+Definition makeForwardAnalysis Dom FunDom (BSL:BoundedSemiLattice Dom)
+         (ftransform : stmt -> (list FunDom * Dom) -> (list FunDom * anni Dom))
+         (fmkFunDom : params -> ann Dom -> FunDom)
+: Analysis (ann Dom) :=
+makeAnalysis _ (fun s d => snd (forward ftransform fmkFunDom s (nil, d))) (fun s => setAnn s bottom).
+
+Definition makeBackwardAnalysis Dom FunDom (BSL:BoundedSemiLattice Dom)
+           (btransform : list FunDom -> stmt -> anni Dom -> Dom)
+           (bmkFunDom : params -> ann Dom -> FunDom)
+: Analysis (ann Dom) :=
+makeAnalysis _
+             (fun s d => backward btransform bmkFunDom s nil d)
+             (fun s => setAnn s bottom).
+
+Section AnalysisAlgorithm.
   Variable Dom : Type.
-  Variable lt : Dom -> Dom -> Prop.
-  Variable lt_dec : forall d d', Computable (lt d d').
+  Variable analysis : Analysis Dom.
+  Hypothesis first : Dom -> (Dom -> Dom * bool) -> Dom.
 
-  Hypothesis first : ann Dom -> (ann Dom -> ann Dom * bool) -> ann Dom.
+  Definition step s (d:Dom) :=
+    let d' := analysis_step analysis s d in
+    (d', if [@poLt_dec _ (dom_po analysis) d' d] then false else true).
 
+  Definition fixpoint (s:stmt) :=
+    first (initial_value analysis s) (step s).
 
-  Context `{AI:AbstractInterpretation Dom}.
-
-  Definition step s d :=
-    let d' := backward AI s nil d in
-    (d', if [ann_R lt d' d] then false else true).
-
-  Definition analysis (s:stmt) :=
-    first (setAnn s bottom) (step s).
-End Analysis.
+End AnalysisAlgorithm.
 
 
 (*
